Add encoder window loop support lemmas

proof/encoder-correctness/VcdiffEnc_Window.thy
@@ -13,9 +13,404 @@ definition encoder_loop_inv :: "byte list \<Rightarrow> nat \<Rightarrow> byte l
   "encoder_loop_inv tgt tp flushed pending \<longleftrightarrow>
      tp \<le> length tgt \<and> flushed @ pending = take tp tgt"
 
+lemma encoder_loop_invI:
+  assumes "tp \<le> length tgt"
+      and "flushed @ pending = take tp tgt"
+  shows "encoder_loop_inv tgt tp flushed pending"
+  using assms by (simp add: encoder_loop_inv_def)
+
 lemma encoder_loop_invD:
   assumes "encoder_loop_inv tgt tp flushed pending"
   shows "tp \<le> length tgt" "flushed @ pending = take tp tgt"
   using assms by (simp_all add: encoder_loop_inv_def)
+
+lemma encoder_loop_inv_tp_le:
+  assumes "encoder_loop_inv tgt tp flushed pending"
+  shows "tp \<le> length tgt"
+  using assms by (simp add: encoder_loop_inv_def)
+
+lemma encoder_loop_inv_prefix_eq:
+  assumes "encoder_loop_inv tgt tp flushed pending"
+  shows "flushed @ pending = take tp tgt"
+  using assms by (simp add: encoder_loop_inv_def)
+
+lemma encoder_loop_inv_lengths:
+  assumes "encoder_loop_inv tgt tp flushed pending"
+  shows "length flushed + length pending = tp"
+proof -
+  have tp_le: "tp \<le> length tgt"
+    and prefix: "flushed @ pending = take tp tgt"
+    using encoder_loop_invD[OF assms] by simp_all
+  have "length flushed + length pending = length (flushed @ pending)"
+    by simp
+  also have "... = length (take tp tgt)"
+    using prefix by simp
+  also have "... = tp"
+    using tp_le by simp
+  finally show ?thesis .
+qed
+
+lemma encoder_loop_inv_flushed_length_le:
+  assumes "encoder_loop_inv tgt tp flushed pending"
+  shows "length flushed \<le> tp"
+  using encoder_loop_inv_lengths[OF assms] by simp
+
+lemma encoder_loop_inv_pending_length_le:
+  assumes "encoder_loop_inv tgt tp flushed pending"
+  shows "length pending \<le> tp"
+  using encoder_loop_inv_lengths[OF assms] by simp
+
+lemma encoder_loop_inv_flushed_eq_take:
+  assumes inv: "encoder_loop_inv tgt tp flushed pending"
+  shows "flushed = take (length flushed) tgt"
+proof -
+  have "flushed = take (length flushed) (flushed @ pending)"
+    by simp
+  also have "... = take (length flushed) (take tp tgt)"
+    using encoder_loop_inv_prefix_eq[OF inv] by simp
+  also have "... = take (length flushed) tgt"
+    using encoder_loop_inv_flushed_length_le[OF inv] by simp
+  finally show ?thesis .
+qed
+
+lemma drop_take_add_eq_take_drop:
+  "drop m (take (m + n) xs) = take n (drop m xs)"
+proof (induction m arbitrary: xs)
+  case 0
+  then show ?case by simp
+next
+  case (Suc m)
+  then show ?case by (cases xs) simp_all
+qed
+
+lemma encoder_loop_inv_pending_eq_drop_take:
+  assumes inv: "encoder_loop_inv tgt tp flushed pending"
+  shows "pending = drop (length flushed) (take tp tgt)"
+proof -
+  have "pending = drop (length flushed) (flushed @ pending)"
+    by simp
+  also have "... = drop (length flushed) (take tp tgt)"
+    using encoder_loop_inv_prefix_eq[OF inv] by simp
+  finally show ?thesis .
+qed
+
+lemma encoder_loop_inv_pending_eq_take_drop:
+  assumes inv: "encoder_loop_inv tgt tp flushed pending"
+  shows "pending = take (length pending) (drop (length flushed) tgt)"
+proof -
+  have len: "length flushed + length pending = tp"
+    by (rule encoder_loop_inv_lengths[OF inv])
+  have "pending = drop (length flushed) (take tp tgt)"
+    by (rule encoder_loop_inv_pending_eq_drop_take[OF inv])
+  also have "... = drop (length flushed)
+      (take (length flushed + length pending) tgt)"
+    using len by simp
+  also have "... = take (length pending) (drop (length flushed) tgt)"
+    by (rule drop_take_add_eq_take_drop)
+  finally show ?thesis .
+qed
+
+lemma encoder_loop_inv_target_prefix:
+  assumes inv: "encoder_loop_inv tgt tp flushed pending"
+  shows "take (length flushed) tgt @ pending = take tp tgt"
+  using encoder_loop_inv_flushed_eq_take[OF inv]
+        encoder_loop_inv_prefix_eq[OF inv]
+  by simp
+
+lemma encoder_loop_inv_empty[simp]:
+  "encoder_loop_inv tgt 0 [] []"
+  by (simp add: encoder_loop_inv_def)
+
+lemma encoder_loop_inv_flush_pending:
+  assumes "encoder_loop_inv tgt tp flushed pending"
+  shows "encoder_loop_inv tgt tp (flushed @ pending) []"
+  using assms by (simp add: encoder_loop_inv_def)
+
+lemma encoder_loop_inv_pending_step:
+  assumes inv: "encoder_loop_inv tgt tp flushed pending"
+      and tp_lt: "tp < length tgt"
+  shows "encoder_loop_inv tgt (Suc tp) flushed (pending @ [tgt ! tp])"
+proof -
+  have "flushed @ (pending @ [tgt ! tp]) = take (Suc tp) tgt"
+    using encoder_loop_inv_prefix_eq[OF inv] tp_lt
+    by (simp add: take_Suc_conv_app_nth)
+  then show ?thesis
+    using tp_lt by (simp add: encoder_loop_inv_def)
+qed
+
+lemma encoder_loop_inv_pending_step_word:
+  fixes tp tgt_len :: "32 word"
+  assumes inv: "encoder_loop_inv tgt (unat tp) flushed pending"
+      and tp_lt: "tp < tgt_len"
+      and tgt_len: "length tgt = unat tgt_len"
+  shows "encoder_loop_inv tgt (unat (tp + 1)) flushed
+           (pending @ [tgt ! unat tp])"
+proof -
+  have tp_nat_lt: "unat tp < length tgt"
+    using tp_lt tgt_len by (simp add: word_less_nat_alt)
+  have tp_suc: "unat (tp + 1) = Suc (unat tp)"
+    using tp_lt by unat_arith
+  show ?thesis
+    using encoder_loop_inv_pending_step[OF inv tp_nat_lt]
+    by (simp add: tp_suc)
+qed
+
+lemma encoder_loop_inv_advance:
+  assumes inv: "encoder_loop_inv tgt tp flushed pending"
+      and adv: "tp + n \<le> length tgt"
+      and chunk: "chunk = take n (drop tp tgt)"
+  shows "encoder_loop_inv tgt (tp + n) (flushed @ pending @ chunk) []"
+proof -
+  have "take (tp + n) tgt = take tp tgt @ take n (drop tp tgt)"
+    by (simp add: take_add)
+  then have "(flushed @ pending @ chunk) @ [] = take (tp + n) tgt"
+    using encoder_loop_inv_prefix_eq[OF inv] chunk by simp
+  then show ?thesis
+    using adv by (simp add: encoder_loop_inv_def)
+qed
+
+lemma encoder_loop_inv_advance_empty_pending:
+  assumes inv: "encoder_loop_inv tgt tp flushed []"
+      and adv: "tp + n \<le> length tgt"
+  shows "encoder_loop_inv tgt (tp + n)
+           (flushed @ take n (drop tp tgt)) []"
+  using encoder_loop_inv_advance[OF inv adv, of "take n (drop tp tgt)"]
+  by simp
+
+lemma encoder_loop_inv_doneD:
+  assumes inv: "encoder_loop_inv tgt tp flushed pending"
+      and tp_done: "tp = length tgt"
+  shows "flushed @ pending = tgt"
+  using encoder_loop_inv_prefix_eq[OF inv] tp_done by simp
+
+lemma encoder_loop_inv_done_no_pendingD:
+  assumes inv: "encoder_loop_inv tgt tp flushed []"
+      and tp_done: "tp = length tgt"
+  shows "flushed = tgt"
+  using encoder_loop_inv_doneD[OF inv tp_done] by simp
+
+lemma match_validD:
+  assumes mv: "match_valid src tgt tp pos len"
+      and len_pos: "0 < len"
+  shows "pos + len \<le> length src"
+        "tp + len \<le> length tgt"
+        "take len (drop pos src) = take len (drop tp tgt)"
+  using mv len_pos by (simp_all add: match_valid_def)
+
+lemma match_valid_take:
+  assumes mv: "match_valid src tgt tp pos len"
+      and n_le: "n \<le> len"
+  shows "match_valid src tgt tp pos n"
+proof (cases "n = 0")
+  case True
+  then show ?thesis by simp
+next
+  case False
+  then have n_pos: "0 < n"
+    by simp
+  then have len_pos: "0 < len"
+    using n_le by simp
+  have src_bound: "pos + len \<le> length src"
+    and tgt_bound: "tp + len \<le> length tgt"
+    and eq: "take len (drop pos src) = take len (drop tp tgt)"
+    using match_validD[OF mv len_pos] by simp_all
+  have "take n (drop pos src) = take n (take len (drop pos src))"
+    using n_le by simp
+  also have "... = take n (take len (drop tp tgt))"
+    using eq by simp
+  also have "... = take n (drop tp tgt)"
+    using n_le by simp
+  finally have take_eq:
+    "take n (drop pos src) = take n (drop tp tgt)" .
+  show ?thesis
+    using src_bound tgt_bound n_le n_pos take_eq
+    by (auto simp: match_valid_def)
+qed
+
+lemma match_valid_drop:
+  assumes mv: "match_valid src tgt tp pos len"
+      and n_le: "n \<le> len"
+  shows "match_valid src tgt (tp + n) (pos + n) (len - n)"
+proof (cases "len = n")
+  case True
+  then show ?thesis by simp
+next
+  case False
+  then have rest_pos: "0 < len - n"
+    using n_le by simp
+  have len_pos: "0 < len"
+    using rest_pos n_le by simp
+  have src_bound: "pos + len \<le> length src"
+    and tgt_bound: "tp + len \<le> length tgt"
+    and eq: "take len (drop pos src) = take len (drop tp tgt)"
+    using match_validD[OF mv len_pos] by simp_all
+  have src_drop:
+    "take (len - n) (drop (pos + n) src) =
+     drop n (take len (drop pos src))"
+    using n_le by (simp add: drop_take drop_drop add.commute)
+  have tgt_drop:
+    "take (len - n) (drop (tp + n) tgt) =
+     drop n (take len (drop tp tgt))"
+    using n_le by (simp add: drop_take drop_drop add.commute)
+  have take_eq:
+    "take (len - n) (drop (pos + n) src) =
+     take (len - n) (drop (tp + n) tgt)"
+    using src_drop tgt_drop eq by simp
+  show ?thesis
+    using src_bound tgt_bound n_le rest_pos take_eq
+    by (auto simp: match_valid_def)
+qed
+
+lemma encoder_loop_inv_advance_match:
+  assumes inv: "encoder_loop_inv tgt tp flushed pending"
+      and mv: "match_valid src tgt tp pos len"
+      and len_pos: "0 < len"
+  shows "encoder_loop_inv tgt (tp + len)
+           (flushed @ pending @ take len (drop pos src)) []"
+proof -
+  have tgt_bound: "tp + len \<le> length tgt"
+    and take_eq: "take len (drop pos src) = take len (drop tp tgt)"
+    using match_validD[OF mv len_pos] by simp_all
+  show ?thesis
+    using encoder_loop_inv_advance[OF inv tgt_bound, of "take len (drop pos src)"]
+          take_eq
+    by simp
+qed
+
+lemma encoder_loop_inv_advance_match_prefix:
+  assumes inv: "encoder_loop_inv tgt tp flushed pending"
+      and mv: "match_valid src tgt tp pos len"
+      and n_pos: "0 < n"
+      and n_le: "n \<le> len"
+  shows "encoder_loop_inv tgt (tp + n)
+           (flushed @ pending @ take n (drop pos src)) []"
+  using encoder_loop_inv_advance_match[OF inv match_valid_take[OF mv n_le] n_pos] .
+
+lemma encoder_loop_inv_advance_match_word:
+  fixes tp len :: "32 word"
+  assumes inv: "encoder_loop_inv tgt (unat tp) flushed pending"
+      and mv: "match_valid src tgt (unat tp) pos (unat len)"
+      and len_pos: "0 < unat len"
+      and no_overflow: "unat tp + unat len < 2 ^ 32"
+  shows "encoder_loop_inv tgt (unat (tp + len))
+           (flushed @ pending @ take (unat len) (drop pos src)) []"
+proof -
+  have tp_len: "unat (tp + len) = unat tp + unat len"
+    using no_overflow by (simp add: unat_word_ariths(1))
+  show ?thesis
+    using encoder_loop_inv_advance_match[OF inv mv len_pos]
+    by (simp add: tp_len)
+qed
+
+lemma section_decodes_empty[simp]:
+  "section_decodes src_seg tgt_len [] [] [] [] cache_init"
+  by (simp add: section_decodes_def section_decodes_prefix_def)
+
+context vcdiff_enc_global_addresses begin
+
+lemma enc_sections_inv_empty:
+  assumes "sections_t_C.data_pos_C sec = 0"
+      and "sections_t_C.inst_pos_C sec = 0"
+      and "sections_t_C.addr_pos_C sec = 0"
+  shows "enc_sections_inv st data inst addr sec src_seg tgt_len
+           [] [] [] [] cache_init"
+  using assms
+  by (simp add: enc_sections_inv_def emitted_sections_def heap_bytes_def)
+
+definition encode_window_c_loop_inv ::
+  "lifted_globals \<Rightarrow>
+   8 word ptr \<Rightarrow> 32 word \<Rightarrow> 8 word ptr \<Rightarrow> 32 word \<Rightarrow>
+   8 word ptr \<Rightarrow> 32 word \<Rightarrow> 8 word ptr \<Rightarrow> 32 word \<Rightarrow>
+   8 word ptr \<Rightarrow> 32 word \<Rightarrow> 8 word ptr \<Rightarrow> 32 word \<Rightarrow>
+   sections_t_C \<Rightarrow> 32 word \<Rightarrow> 32 word \<Rightarrow>
+   byte list \<Rightarrow> byte list \<Rightarrow> byte list \<Rightarrow> byte list \<Rightarrow> byte list \<Rightarrow>
+   byte list \<Rightarrow> byte list \<Rightarrow> cache \<Rightarrow> bool" where
+  "encode_window_c_loop_inv st
+     src src_len tgt tgt_len data data_cap inst inst_cap addr addr_cap
+     pending pending_cap sec tp pend_len
+     src_seg tgt_bytes data_bytes inst_bytes addr_bytes
+     flushed pending_bytes c_out \<longleftrightarrow>
+     sections_t_C.err_C sec = ENC_OK \<and>
+     length src_seg = unat src_len \<and>
+     length tgt_bytes = unat tgt_len \<and>
+     heap_bytes st src (length src_seg) = src_seg \<and>
+     heap_bytes st tgt (length tgt_bytes) = tgt_bytes \<and>
+     heap_bytes st pending (unat pend_len) = pending_bytes \<and>
+     length pending_bytes = unat pend_len \<and>
+     unat pend_len \<le> unat pending_cap \<and>
+     unat (sections_t_C.data_pos_C sec) \<le> unat data_cap \<and>
+     unat (sections_t_C.inst_pos_C sec) \<le> unat inst_cap \<and>
+     unat (sections_t_C.addr_pos_C sec) \<le> unat addr_cap \<and>
+     encoder_loop_inv tgt_bytes (unat tp) flushed pending_bytes \<and>
+     enc_sections_inv st data inst addr sec src_seg (length tgt_bytes)
+       data_bytes inst_bytes addr_bytes flushed c_out"
+
+lemma encode_window_c_loop_invD:
+  assumes inv: "encode_window_c_loop_inv st
+     src src_len tgt tgt_len data data_cap inst inst_cap addr addr_cap
+     pending pending_cap sec tp pend_len
+     src_seg tgt_bytes data_bytes inst_bytes addr_bytes
+     flushed pending_bytes c_out"
+  shows "sections_t_C.err_C sec = ENC_OK"
+        "length src_seg = unat src_len"
+        "length tgt_bytes = unat tgt_len"
+        "heap_bytes st src (length src_seg) = src_seg"
+        "heap_bytes st tgt (length tgt_bytes) = tgt_bytes"
+        "heap_bytes st pending (unat pend_len) = pending_bytes"
+        "length pending_bytes = unat pend_len"
+        "unat pend_len \<le> unat pending_cap"
+        "unat (sections_t_C.data_pos_C sec) \<le> unat data_cap"
+        "unat (sections_t_C.inst_pos_C sec) \<le> unat inst_cap"
+        "unat (sections_t_C.addr_pos_C sec) \<le> unat addr_cap"
+        "encoder_loop_inv tgt_bytes (unat tp) flushed pending_bytes"
+        "enc_sections_inv st data inst addr sec src_seg (length tgt_bytes)
+           data_bytes inst_bytes addr_bytes flushed c_out"
+  using inv by (auto simp: encode_window_c_loop_inv_def)
+
+lemma encode_window_c_loop_inv_tp_le_tgt_len:
+  assumes inv: "encode_window_c_loop_inv st
+     src src_len tgt tgt_len data data_cap inst inst_cap addr addr_cap
+     pending pending_cap sec tp pend_len
+     src_seg tgt_bytes data_bytes inst_bytes addr_bytes
+     flushed pending_bytes c_out"
+  shows "unat tp \<le> unat tgt_len"
+  using encode_window_c_loop_invD(3,12)[OF inv]
+        encoder_loop_inv_tp_le[of tgt_bytes "unat tp" flushed pending_bytes]
+  by simp
+
+lemma encode_window_c_loop_inv_prefix_eq:
+  assumes inv: "encode_window_c_loop_inv st
+     src src_len tgt tgt_len data data_cap inst inst_cap addr addr_cap
+     pending pending_cap sec tp pend_len
+     src_seg tgt_bytes data_bytes inst_bytes addr_bytes
+     flushed pending_bytes c_out"
+  shows "flushed @ pending_bytes = take (unat tp) tgt_bytes"
+  using encode_window_c_loop_invD(12)[OF inv]
+  by (rule encoder_loop_inv_prefix_eq)
+
+lemma encode_window_c_loop_inv_entry:
+  assumes sec: "sections_result sec 0 0 0 ENC_OK"
+      and src_len: "length src_seg = unat src_len"
+      and tgt_len: "length tgt_bytes = unat tgt_len"
+      and src_heap: "heap_bytes st src (length src_seg) = src_seg"
+      and tgt_heap: "heap_bytes st tgt (length tgt_bytes) = tgt_bytes"
+  shows "encode_window_c_loop_inv st
+     src src_len tgt tgt_len data data_cap inst inst_cap addr addr_cap
+     pending pending_cap sec 0 0
+     src_seg tgt_bytes [] [] [] [] [] cache_init"
+proof -
+  have sec_fields:
+    "sections_t_C.data_pos_C sec = 0"
+    "sections_t_C.inst_pos_C sec = 0"
+    "sections_t_C.addr_pos_C sec = 0"
+    "sections_t_C.err_C sec = ENC_OK"
+    using sections_resultD[OF sec] by simp_all
+  show ?thesis
+    using src_len tgt_len src_heap tgt_heap sec_fields
+          enc_sections_inv_empty[of sec st data inst addr src_seg "length tgt_bytes"]
+    by (simp add: encode_window_c_loop_inv_def heap_bytes_def)
+qed
+
+end
 
 end
